DY/Actions/LongTermKeys.lean
@@ -1,0 +1,453 @@
+module
+
+public import DY.Trace
+public import DY.Bytes
+public import DY.Actions.Random
+public import DY.Actions.Network
+public import DY.Actions.PersistentGlobalState
+public import DY.Actions.PersistentLocalState
+import DY.Step.Init
+
+namespace DY.LongTermKeys
+
+section Execution
+
+public
+class ExecConfig [BytesFunctor] (name: String) (skToPk: outParam (Bytes → Bytes)) where
+
+public
+structure SecretKeyState [BytesFunctor] (name: String) where
+  sk: Bytes
+
+public
+noncomputable
+instance [BytesFunctor] (name: String): Comparse.ParseableSerializeable (SecretKeyState name) := Comparse.comparseMetaProgramExists
+
+public
+structure PublicKeyState [BytesFunctor] (name: String) where
+  p: Participant
+  pk: Bytes
+
+public
+noncomputable
+instance [BytesFunctor] (name: String): Comparse.ParseableSerializeable (PublicKeyState name) := Comparse.comparseMetaProgramExists
+
+variable [BytesFunctor]
+variable (name: String)
+variable {skToPk: Bytes → Bytes}
+variable [ExecConfig name skToPk]
+
+@[expose, implicit_reducible]
+public
+def ExecEntryT.internal: Fin 2 → Type
+  | 0 => PersistentLocalState.CompromisableState.ExecEntryT (SecretKeyState name)
+  | 1 => PersistentGlobalState.CompromisableState.ExecEntryT (PublicKeyState name)
+
+@[expose, implicit_reducible]
+public
+def ExecEntryT: Type :=
+  ExecTraceTypes.combine (ExecEntryT.internal name)
+
+public
+instance: ExecTraceTypes.HasStep (PersistentLocalState.CompromisableState.ExecEntryT (SecretKeyState name)) (ExecEntryT name) :=
+  inferInstanceAs (ExecTraceTypes.HasStep (ExecEntryT.internal name 0) (ExecTraceTypes.combine (ExecEntryT.internal name)))
+
+public
+instance: ExecTraceTypes.HasStep (PersistentGlobalState.CompromisableState.ExecEntryT (PublicKeyState name)) (ExecEntryT name) :=
+  inferInstanceAs (ExecTraceTypes.HasStep (ExecEntryT.internal name 1) (ExecTraceTypes.combine (ExecEntryT.internal name)))
+
+public
+def baseAttackerKnowledge.internal [ExecTraceTypes]: (id: Fin 2) → SubBaseAttackerKnowledge (ExecEntryT.internal name id)
+  | 0 => PersistentLocalState.CompromisableState.baseAttackerKnowledge (SecretKeyState name)
+  | 1 => PersistentGlobalState.CompromisableState.baseAttackerKnowledge (PublicKeyState name)
+
+public
+def baseAttackerKnowledge  [ExecTraceTypes]: SubBaseAttackerKnowledge (ExecEntryT name) :=
+  SubBaseAttackerKnowledge.combine (baseAttackerKnowledge.internal name)
+
+public
+def generateKeyPair
+  [ExecConfig name skToPk]
+  [ExecTraceTypes]
+  [BytesFunctor.Has Random.SubF]
+  [ExecTraceTypes.Has Random.ExecEntryT]
+  [ExecTraceTypes.Has Network.ExecEntryT]
+  [ExecTraceTypes.Has <| ExecEntryT name]
+  (p: Participant)
+  : Traceful (Nat × Nat × Nat)
+:= do
+  let sk ← Random.genRand 32
+  let pk := skToPk sk
+  let tsMsg ← Network.sendMessage pk
+  let tsPk ← PersistentGlobalState.storeGlobalState ({p, pk}: PublicKeyState name)
+  let tsSk ← PersistentLocalState.storeLocalState p ({sk}: SecretKeyState name)
+  pure (tsMsg, tsPk, tsSk)
+
+public
+def getPublicKey
+  [ExecTraceTypes]
+  [ExecTraceTypes.Has <| ExecEntryT name]
+  (p: Participant)
+  (tsPk: Nat)
+  : Traceful Bytes
+:= do
+  let st: PublicKeyState name ← PersistentGlobalState.getGlobalState tsPk
+  guard (st.p = p)
+  pure st.pk
+
+public
+def getPrivateKey
+  [ExecTraceTypes]
+  [ExecTraceTypes.Has <| ExecEntryT name]
+  (p: Participant)
+  (tsSk: Nat)
+  : Traceful Bytes
+:= do
+  let st: SecretKeyState name ← PersistentLocalState.getLocalState p tsSk
+  pure st.sk
+
+public
+def LongTermKeyCompromised
+  [ExecConfig name skToPk] [ExecTraceTypes] [ExecTraceTypes.Has (ExecEntryT name)]
+  (participant: Participant) (pk: Bytes)
+  (tr: ExecTrace)
+  : Prop
+:=
+  ∃ sk,
+    pk = skToPk sk ∧
+    PersistentLocalState.LocalStateCompromised participant ({ sk }: SecretKeyState name) tr
+
+public
+theorem LongTermKeyCompromised_le
+  [ExecTraceTypes] [ExecTraceTypes.Has (ExecEntryT name)]
+  (participant: Participant) (pk: Bytes)
+  (tr1 tr2: ExecTrace)
+  : tr1 ≤ tr2 →
+    LongTermKeyCompromised name participant pk tr1 →
+    LongTermKeyCompromised name participant pk tr2
+:= by
+  simp [LongTermKeyCompromised]
+  grind
+
+grind_pattern LongTermKeyCompromised_le => tr1 ≤ tr2, LongTermKeyCompromised name participant pk tr1
+grind_pattern [grind_later] LongTermKeyCompromised_le => tr1 ≤ tr2, LongTermKeyCompromised name participant pk tr1
+
+end Execution
+
+section Proof
+
+@[expose]
+public
+def label
+  [BytesFunctor]
+  (name: String) {skToPk: Bytes → Bytes} [ExecConfig name skToPk]
+  [ExecTraceTypes] [ExecTraceTypes.Has (ExecEntryT name)]
+  (participant: Participant) (pk: Bytes)
+  : Label
+where
+  isCorrupt := LongTermKeyCompromised name participant pk
+
+public
+class ProofConfig
+  [BytesFunctor] [TraceTypes] [BytesInvariants]
+  (name: String) {skToPk: outParam (Bytes → Bytes)} (usage: outParam (Participant → Usage))
+  [ExecConfig name skToPk]
+  [ExecTraceTypes.Has (ExecEntryT name)]
+where
+  IsLongTermPublicKey: Participant → Bytes → ProofTrace → Prop
+
+  IsLongTermPublicKey_le: ∀ p b tr1 tr2,
+    tr1 ≤ tr2 →
+    IsLongTermPublicKey p b tr1 →
+    IsLongTermPublicKey p b tr2
+  := by grind
+
+  IsLongTermPublicKey_implied (name): ∀ p b tr,
+    b.Invariant tr →
+    b.label tr = label name p (skToPk b) →
+    b.HasUsage (usage p) tr →
+    IsLongTermPublicKey p (skToPk b) tr
+
+  IsLongTermPublicKey_implies (name): ∀ p b tr,
+    IsLongTermPublicKey p b tr →
+    b.Publishable tr
+  := by grind
+
+export ProofConfig (IsLongTermPublicKey)
+
+grind_pattern ProofConfig.IsLongTermPublicKey_le => tr1 ≤ tr2, ProofConfig.IsLongTermPublicKey name p b tr1
+grind_pattern [grind_later] ProofConfig.IsLongTermPublicKey_le => tr1 ≤ tr2, ProofConfig.IsLongTermPublicKey name p b tr1
+
+public
+theorem IsLongTermPublicKey_implies_Invariant
+  [BytesFunctor] [TraceTypes] [BytesInvariants]
+  (name: String) {skToPk: Bytes → Bytes} (usage: Participant → Usage)
+  [ExecTraceTypes.Has (ExecEntryT name)]
+  [ExecConfig name skToPk] [ProofConfig name usage]
+  (p: Participant) (b: Bytes) (tr: ProofTrace)
+  : IsLongTermPublicKey name p b tr →
+    b.Invariant tr
+:= by
+  have := ProofConfig.IsLongTermPublicKey_implies name
+  grind
+
+grind_pattern [grind_later] IsLongTermPublicKey_implies_Invariant => IsLongTermPublicKey name p b tr
+
+@[expose]
+public
+def IsLongTermSecretKey
+  [BytesFunctor] [TraceTypes] [BytesInvariants]
+  (name: String) {skToPk: Bytes → Bytes} {usage: Participant → Usage}
+  [ExecTraceTypes.Has (ExecEntryT name)]
+  [ExecConfig name skToPk] [ProofConfig name usage]
+  (p: Participant) (b: Bytes) (tr: ProofTrace)
+  : Prop
+:=
+  b.Invariant tr ∧
+  b.label tr = label name p (skToPk b) ∧
+  b.HasUsage (usage p) tr
+
+public
+theorem IsLongTermSecretKey_later
+  [BytesFunctor] [TraceTypes] [BytesInvariants] [BytesInvariantsProofs]
+  (name: String) {skToPk: Bytes → Bytes} {usage: Participant → Usage}
+  [ExecTraceTypes.Has (ExecEntryT name)]
+  [ExecConfig name skToPk] [ProofConfig name usage]
+  (p: Participant) (b: Bytes) (tr1 tr2: ProofTrace)
+  : tr1 ≤ tr2 →
+    IsLongTermSecretKey name p b tr1 →
+    IsLongTermSecretKey name p b tr2
+:= by
+  grind [IsLongTermSecretKey]
+
+grind_pattern [grind_later] IsLongTermSecretKey_later => tr1 ≤ tr2, IsLongTermSecretKey name p b tr1
+
+axiom SecretKeyState.isWellFormedLemma
+  [BytesFunctor]
+  (pre: Bytes → τ → Prop) [Comparse.BytesCompatible pre]
+  (x: SecretKeyState name) (tr: τ):
+  Comparse.isWellFormed pre x tr = pre x.sk tr
+
+grind_pattern SecretKeyState.isWellFormedLemma => Comparse.isWellFormed pre x tr
+
+axiom PublicKeyState.isWellFormedLemma
+  [BytesFunctor]
+  (pre: Bytes → τ → Prop) [Comparse.BytesCompatible pre]
+  (x: PublicKeyState name) (tr: τ):
+  Comparse.isWellFormed pre x tr = pre x.pk tr
+
+grind_pattern PublicKeyState.isWellFormedLemma => Comparse.isWellFormed pre x tr
+
+section
+
+variable [BytesFunctor] [TraceTypes] [BytesInvariants] [BytesInvariantsProofs]
+variable (name: String)
+variable [ExecTraceTypes.Has <| ExecEntryT name]
+variable {skToPk: Bytes → Bytes} {usage: Participant → Usage}
+variable [ExecConfig name skToPk] [ProofConfig name usage]
+
+public
+instance [ProofConfig name usage]: PersistentLocalState.CompromisableLocalStateInv (SecretKeyState name) where
+  invariant p st tr :=
+    IsLongTermSecretKey name p st.sk tr
+  invariant_later := by grind [IsLongTermSecretKey]
+  invariant_implies_KnowableBy := by
+    intro participant state tr h
+    have: (label name participant (skToPk state.sk)).canFlow (PersistentLocalState.label participant state) tr.erase := by
+      cases state
+      simp [Label.canFlow, label, LongTermKeyCompromised, PersistentLocalState.label_isCorrupt]
+      grind
+    grind [canFlowTrans, IsLongTermSecretKey]
+
+public
+instance: PersistentGlobalState.CompromisableGlobalStateInv (PublicKeyState name) where
+  invariant st tr :=
+    IsLongTermPublicKey name st.p st.pk tr
+  invariant_later := by grind [ProofConfig.IsLongTermPublicKey_le]
+  invariant_implies_KnowableBy := by
+    intro state tr h
+    have := ProofConfig.IsLongTermPublicKey_implies name state.p state.pk tr h
+    grind [canFlowTrans]
+
+@[expose, implicit_reducible]
+public
+def ProofEntryT.internal: Fin 2 → Type
+  | 0 => PersistentLocalState.CompromisableState.ProofEntryT (SecretKeyState name)
+  | 1 => PersistentGlobalState.CompromisableState.ProofEntryT (PublicKeyState name)
+
+@[expose, implicit_reducible]
+public
+def ProofEntryT: Type :=
+  TraceTypes.combine (ProofEntryT.internal name)
+
+public
+instance: ∀ id, ErasableProofEntry (ExecEntryT.internal name id) (ProofEntryT.internal name id)
+  | 0 | 1 => by dsimp only [ExecEntryT.internal, ProofEntryT.internal]; infer_instance
+
+public
+instance: ErasableProofEntry (ExecEntryT name) (ProofEntryT name) :=
+  (inferInstance: ErasableProofEntry (ExecTraceTypes.combine (ExecEntryT.internal name)) (TraceTypes.combine (ProofEntryT.internal name)))
+
+public
+instance: TraceTypes.HasStep (PersistentLocalState.CompromisableState.ProofEntryT (SecretKeyState name)) (ProofEntryT name) :=
+  inferInstanceAs (TraceTypes.HasStep (ProofEntryT.internal name 0) (TraceTypes.combine (ProofEntryT.internal name)))
+
+public
+instance: TraceTypes.HasStep (PersistentGlobalState.CompromisableState.ProofEntryT (PublicKeyState name)) (ProofEntryT name) :=
+  inferInstanceAs (TraceTypes.HasStep (ProofEntryT.internal name 1) (TraceTypes.combine (ProofEntryT.internal name)))
+
+public
+noncomputable
+instance
+  : ∀ id, ProofEntryInvariant (ProofEntryT.internal name id)
+  | 0 | 1 => by dsimp only [ProofEntryT.internal]; infer_instance
+
+public
+noncomputable
+instance
+  : ProofEntryInvariant (ProofEntryT name)
+:=
+  (inferInstance: ProofEntryInvariant (TraceTypes.combine (ProofEntryT.internal name)))
+
+public
+instance
+  : TraceInvariant.HasStep (PersistentLocalState.CompromisableState.ProofEntryT (SecretKeyState name)) (ProofEntryT name)
+:=
+  inferInstanceAs (TraceInvariant.HasStep (ProofEntryT.internal name 0) (TraceTypes.combine (ProofEntryT.internal name)))
+
+public
+instance
+  : TraceInvariant.HasStep (PersistentGlobalState.CompromisableState.ProofEntryT (PublicKeyState name)) (ProofEntryT name)
+:=
+  inferInstanceAs (TraceInvariant.HasStep (ProofEntryT.internal name 1) (TraceTypes.combine (ProofEntryT.internal name)))
+
+end
+
+section
+
+public
+instance
+  [BytesFunctor] [TraceInvariant] [BytesInvariants] [BytesInvariantsProofs]
+  [TraceTypes.Has (ProofEntryT name)]
+  {skToPk: Bytes → Bytes} {usage: Participant → Usage}
+  [ExecConfig name skToPk] [ProofConfig name usage]
+  [TraceInvariant.Has (ProofEntryT name)]
+  : ∀ id, SubBaseAttackerKnowledgeTheorem (ProofEntryT.internal name id) (baseAttackerKnowledge.internal name id)
+  -- TODO: investigate why infer_instance doesn't work
+  | 0 => by dsimp only [ProofEntryT.internal, baseAttackerKnowledge.internal]; apply PersistentLocalState.CompromisableState.baseAttackerKnowledgeTheorem
+  | 1 => by dsimp only [ProofEntryT.internal, baseAttackerKnowledge.internal]; apply PersistentGlobalState.CompromisableState.baseAttackerKnowledgeTheorem
+
+public
+instance baseAttackerKnowledgeTheorem
+  [BytesFunctor] [TraceInvariant] [BytesInvariants] [BytesInvariantsProofs]
+  (name: String) {skToPk: Bytes → Bytes} {usage: Participant → Usage}
+  [TraceTypes.Has (ProofEntryT name)]
+  [ExecConfig name skToPk] [ProofConfig name usage]
+  [TraceInvariant.Has (ProofEntryT name)]
+  : SubBaseAttackerKnowledgeTheorem (ProofEntryT name) (baseAttackerKnowledge name)
+:= by
+  dsimp only [ProofEntryT, baseAttackerKnowledge]
+  apply instSubBaseAttackerKnowledgeTheoremCombine -- infer_instance?
+
+end
+
+@[instance]
+public
+theorem generateKeyPair.spec
+  [BytesFunctor]
+  [TraceInvariant]
+  [BytesInvariants] [BytesInvariantsProofs]
+
+  (name: String)
+  {skToPk: Bytes → Bytes} {usage: Participant → Usage}
+
+  [BytesFunctor.Has Random.SubF]
+
+  [TraceTypes.Has <| Random.ProofEntryT]
+  [TraceTypes.Has <| Network.ProofEntryT]
+  [TraceTypes.Has <| ProofEntryT name]
+
+  [BytesInvariants.Has <| Random.invariants]
+
+  [ExecConfig name skToPk] [ProofConfig name usage]
+  [TraceInvariant.Has <| Random.ProofEntryT]
+  [TraceInvariant.Has <| Network.ProofEntryT]
+  [TraceInvariant.Has <| ProofEntryT name]
+  (p: Participant)
+  : HoareTriple
+    (generateKeyPair name p)
+    (fun _ => True)
+    (fun _ _ => True)
+:= by
+  unfold generateKeyPair
+  dsimp only
+  step with ⟨ fun sk => label name p (skToPk sk), usage p ⟩
+  step by
+    have := ProofConfig.IsLongTermPublicKey_implied name
+    have := ProofConfig.IsLongTermPublicKey_implies name
+    grind
+  step by
+    have := ProofConfig.IsLongTermPublicKey_implied name
+    simp [PersistentGlobalState.GlobalStateInv.invariant]
+    grind
+  step by
+    have := ProofConfig.IsLongTermPublicKey_implied name
+    simp [PersistentLocalState.LocalStateInv.invariant, IsLongTermSecretKey]
+    grind
+  step
+  trivial
+
+@[instance]
+public
+theorem getPublicKey.spec
+  [BytesFunctor]
+  [TraceInvariant]
+  [BytesInvariants] [BytesInvariantsProofs]
+
+  (name: String)
+  {skToPk: Bytes → Bytes} {usage: Participant → Usage}
+
+  [BytesFunctor.Has Random.SubF]
+  [TraceTypes.Has <| ProofEntryT name]
+  [ExecConfig name skToPk] [ProofConfig name usage]
+  [TraceInvariant.Has <| ProofEntryT name]
+  (p: Participant)
+  : HoareTriple
+    (getPublicKey name p tsPk)
+    (fun _ => True)
+    (fun res tr => ProofConfig.IsLongTermPublicKey name p res tr)
+:= by
+  unfold getPublicKey
+  step
+  step
+  step
+  simp_all [PersistentGlobalState.GlobalStateInv.invariant]
+
+@[instance]
+public
+theorem getPrivateKey.spec
+  [BytesFunctor]
+  [TraceInvariant]
+  [BytesInvariants] [BytesInvariantsProofs]
+
+  (name: String)
+  {skToPk: Bytes → Bytes} {usage: Participant → Usage}
+
+  [BytesFunctor.Has Random.SubF]
+  [TraceTypes.Has <| ProofEntryT name]
+  [ExecConfig name skToPk] [ProofConfig name usage]
+  [TraceInvariant.Has <| ProofEntryT name]
+  (p: Participant)
+  : HoareTriple
+    (getPrivateKey name p tsSk)
+    (fun _ => True)
+    (fun res tr => IsLongTermSecretKey name p res tr)
+:= by
+  unfold getPrivateKey
+  step
+  step
+  simp_all [PersistentLocalState.LocalStateInv.invariant, IsLongTermSecretKey]
+
+end Proof
+
+end DY.LongTermKeys
